io/ho_examples/Callback.Level1.fst
@@ -1,0 +1,91 @@
+module Callback.Level1
+
+open FStar.Tactics
+
+open Common
+open DM 
+open TC.ML
+open TC.ML.HO
+open TC.Checkable
+open TC.Export
+open TC.MLify.IIOwp
+open TC.Monitorable.Hist
+open TC.Instrumentable.IIOwp
+
+(** ***  accepts a function that accepts a callback **)
+(** pp  - partial program (TRUSTED)
+    ctx - context         (UNTRUSTED)
+    pp_cb - callback of partial program (TRUSTED) **)
+
+assume val pi : monitorable_prop
+
+(** The type of the callback function.
+    The callback function in this example has non-higher-order types as input and output.
+    The callback is TRUSTED and it is passed by the main function to the UNTRUSTED side.
+    Thus, callback must be mlified before being past to the UNTRUSTED side.
+    Because the callback function is mlified, it means that the runtime checks can fail.
+    Because the UNTRUSTED side is instrumented to respect pi --- meaning that the post-conditon
+    of the UNTRUSTED side guarantees pi is respected --- the callback has also to respect pi.
+    Therefore, the callback function can be mlified only if it is part of the class mlifyable_guarded.
+**)
+assume val pp_cb_in  : Type
+assume val pp_cb_in_importable : importable pp_cb_in
+assume val pp_cb_out : Type
+assume val pp_cb_out_exportable : exportable pp_cb_out
+assume val pp_cb_pre : pp_cb_in -> trace -> Type0
+assume val pp_cb_post : pp_cb_in -> trace -> maybe pp_cb_out -> trace -> Type0
+type pp_cb = x:pp_cb_in -> IIO (maybe pp_cb_out) (pp_cb_pre x) (pp_cb_post x) 
+
+(** The UNTRUSTED side accepts the callback.
+    The UNTRUSTED side expects a callback that can fail.
+    Its pre-condition is a promise, thus is not verified dynamically.
+    Since the UNTRUSTED side is instrumented and its post-condition is dynamically
+    enforced, its output type must reflect the possibility of a contract failure.
+**)
+assume val ctx_out : Type
+assume val ctx_out_importable : importable (maybe ctx_out)
+assume val ctx_pre : trace -> Type0
+assume val ctx_post : trace -> maybe ctx_out -> trace -> Type0
+type ctx = pp_cb -> IIO (maybe ctx_out) ctx_pre ctx_post 
+
+assume val pp_out : Type
+assume val pp_out_exportable : exportable pp_out
+assume val pp_pre : trace -> Type0
+assume val pp_post : trace -> maybe pp_out -> trace -> Type0
+type pp = ctx -> IIO (maybe pp_out) pp_pre pp_post
+
+assume val pp_cb_pre_checkable : checkable2 pp_cb_pre
+assume val pp_cb_post_cpi : squash (forall x h lt r. pp_cb_pre x h /\ pp_cb_post x h r lt ==> enforced_locally pi h lt)
+
+
+let pp_cb_mlifyable_guarded : mlifyable_guarded pp_cb_in pp_cb_out pp_cb_pre pp_cb_post pi = {
+  cmlifyable = mlifyable_iiowp_trivialize_weaken_post pp_cb_in #pp_cb_in_importable pp_cb_out #pp_cb_out_exportable pp_cb_pre #pp_cb_pre_checkable pp_cb_post;
+  cpi = pp_cb_post_cpi
+}
+
+assume val ctx_post_monitorable : monitorable_post #pp_cb_mlifyable_guarded.cmlifyable.matype (fun x -> ctx_pre) (fun x -> ctx_post) pi
+
+let ctx_instrumentable : instrumentable ctx =
+  instrumentable_HO pp_cb_in pp_cb_out pp_cb_pre pp_cb_post ctx_out ctx_pre ctx_post pi
+  #ctx_out_importable
+  #pp_cb_mlifyable_guarded
+  #ctx_post_monitorable
+
+
+assume val pp_pre_checkable : checkable pp_pre
+  
+let pp_mlifyable : mlifyable pp =
+  mlifyable_inst_iiowp_trivialize_weaken ctx #ctx_instrumentable pp_out #pp_out_exportable pp_pre #pp_pre_checkable pp_post 
+
+let test_output_type (main:pp) : (((pp_cb_in_importable.itype -> MIIO (maybe (pp_cb_out_exportable.etype))) -> IIOpi (ctx_out_importable.itype) pi) -> MIIO (maybe (pp_out_exportable.etype)))
+  by (unfold_def (`Mkmlifyable?.matype); unfold_def (`Mkmlifyable_guarded?.cmlifyable); rewrite_eqs_from_context (); norm [iota]; 
+  explode ();
+  bump_nth 5;
+//  dump "H";
+  tadmit ()
+  )=
+  mlify #_ #(mlifyable_inst_iiowp_trivialize_weaken ctx #ctx_instrumentable pp_out #pp_out_exportable pp_pre #pp_pre_checkable pp_post) main
+
+(** CA: I don't like in this example that every output type contains maybe.
+    It is necessary to have this for cb and f because our effect does not support halting the execution
+    when a contract failure occurs. **)
